Refinery/Term/Extrinsic/Semantics/Minimal.lean
@@ -31,9 +31,9 @@ def SDeriv.den {Γ : Ctx? α} {A : Ty α} {a : Term φ (Ty α)}
     ≫ _ ◁ dqb.den ≫ db.den
   | .inl da => da.den ≫ CC.inl _ _
   | .inr db => db.den ≫ CC.inr _ _
-  | .case dΓ dqa dqb da db dc =>
+  | .case dΓ dΓl dqa dqb da db dc =>
     dΓ.den ≫ (_ ◁ da.den) ≫ (∂L _ _ _).inv
-           ≫ desc (_ ◁ dqa.den ≫ db.den) (_ ◁ dqb.den ≫ dc.den)
+           ≫ desc ((dΓl.zwkLeft.den ⊗ dqa.den) ≫ db.den) ((dΓl.zwkRight.den ⊗ dqb.den) ≫ dc.den)
   | .abort da => da.den ≫ CC.fromZero _
   | .iter (A := A) (B := B) (Γl := Γl) dΓ dq _ _ da db =>
     dΓ.den ≫ (_ ◁ da.den) ≫ iterate (
@@ -56,18 +56,36 @@ theorem SDeriv.den_cast_term {Γ : Ctx? α} {A : Ty α} {a a' : Term φ (Ty α)}
 
 theorem SDeriv.den_unstrict {Γ : Ctx? α} {A : Ty α} {a : Term φ (Ty α)} (D : Γ ⊢ₛ a : A)
   : D.unstrict.den = D.den (C := C) := by
-  induction D
-  <;> simp [den, unstrict, Deriv.den, Deriv.den_pwk, tensorHom_def, Ctx?.SAt.den_unstrict, *]
+  induction D <;> simp [
+    den, unstrict, Deriv.den, Deriv.den_pwk, tensorHom_def, Ctx?.SAt.den_unstrict,
+    Ctx?.ZWk.den_toPWk, *]
 
--- theorem SDeriv.coherence {Γ : Ctx? α} {A : Ty α} {a : Term φ (Ty α)}
---   (D D' : Γ ⊢ₛ a : A) : D.den (C := C) = D'.den := by induction D with
---   | bv x => cases D' with | bv x' => rw [Subsingleton.elim x x']
---   | op hf => cases D' with | op hf' =>
---     cases hf.trg; cases hf'.trg; cases hf.src; cases hf'.src
---     simp only [den]; congr 1; apply_assumption
---   | let₁ =>
---     cases D'
---     simp only [den]
---     rename Ctx?.SSplit _ _ _ => hΓ
---     sorry
---   | _ => sorry
+def FDeriv.den {Γ : Ctx? α} {A : Ty α} {a : Term φ (Ty α)} (D : Γ ⊢ₛ' a : A)
+  : (g⟦ Γ ⟧ : C) ⟶ t⟦ A ⟧ := D.drop.den ≫ D.deriv.den
+
+theorem FDeriv.den_toDeriv {Γ : Ctx? α} {A : Ty α} {a : Term φ (Ty α)} (D : Γ ⊢ₛ' a : A)
+  : D.toDeriv.den (C := C) = D.den := by simp only [toDeriv, Deriv.den_pwk, Ctx?.ZWk.den_toPWk,
+    SDeriv.den_unstrict, den]
+
+theorem SDeriv.coherence {Γ : Ctx? α} {A : Ty α} {a : Term φ (Ty α)}
+  (D D' : Γ ⊢ₛ a : A) : D.den (C := C) = D'.den := by induction D with
+  | bv x => cases D' with | bv x' => rw [Subsingleton.elim x x']
+  | op hf => cases D' with | op hf' =>
+    cases hf.trg; cases hf'.trg; cases hf.src; cases hf'.src
+    simp only [den]; congr 1; apply_assumption
+  | let₁ =>
+    cases D'
+    simp only [den]
+    rename Ctx?.SSplit _ _ _ => hΓ
+    sorry
+  | _ => sorry
+
+theorem FDeriv.coherence {Γ : Ctx? α} {A : Ty α} {a : Term φ (Ty α)}
+  (D D' : Γ ⊢ₛ' a : A) : D.den (C := C) = D'.den := sorry
+
+theorem Deriv.den_factor {Γ : Ctx? α} {A : Ty α} {a : Term φ (Ty α)} (D : Γ ⊢ a : A)
+  : D.factor.den (C := C) = D.den := sorry
+
+theorem Deriv.coherence {Γ : Ctx? α} {A : Ty α} {a : Term φ (Ty α)}
+  (D D' : Γ ⊢ a : A) : D.den (C := C) = D'.den
+  := by rw [<-D.den_factor, <-D'.den_factor, D.factor.coherence D'.factor]
